Temporary implementation of br_reduce and return_reduce

spectec/test-coq/theories/type_progress.v
@@ -413,15 +413,15 @@ Lemma list_slice_size : forall {T : Type} (bs : seq T) i j,
 Proof.
   move => T bs.
   elim: bs => [| b bs' IH].
-  + move => /= i j H.
+  - move => /= i j H.
     have H' := leq_addl i j.
     move: (leq_trans H' H) => {}H.
     rewrite (leqn0 j) in H.
     by move/eqP in H.
-  + move => /= i j H.
+  - move => /= i j H.
     case: i H => [| i'] H; case: j H => [| j'] H //=.
-    * congr S. by apply: IH.
-    * apply: IH.
+    + congr S. by apply: IH.
+    + apply: IH.
       rewrite -[i'.+1]addn1 -[(size bs').+1]addn1 in H.
       rewrite -addnA -[1 + j'.+1]addnC addnA in H.
       by rewrite (leq_add2r 1) in H.
@@ -439,6 +439,169 @@ Axiom fun_ibytes_inverse : forall n bs,
 Scheme Instr_ok_ind' := Induction for Instr_ok Sort Prop
   with Instrs_ok_ind' := Induction for Instrs_ok Sort Prop.
 
+Definition br_reduce es := 
+  exists vcs l es',
+  es = list__val__admininstr vcs ++ [:: admininstr__BR l] ++ es'.
+
+Definition return_reduce es :=
+  exists vcs es',
+  es = list__val__admininstr vcs ++ [:: admininstr__RETURN] ++ es'.
+
+(* NOTE: We could define this as ~ (br_reduce es) *)
+Definition not_lf_br es :=
+  forall vcs l es',
+  es <> list__val__admininstr vcs ++ [:: admininstr__BR l] ++ es'.
+
+(* NOTE: We could define this as ~ (br_reduce es) *)
+Definition not_lf_return es :=
+  forall vcs es',
+  es <> list__val__admininstr vcs ++ [:: admininstr__RETURN] ++ es'.
+
+(* TODO: Define this in generatedcode.v *)
+Fixpoint split_vals (es : seq admininstr) : seq (generatedcode.val) * seq admininstr :=
+  match es with
+  | (admininstr__CONST t v) :: es' =>
+    let: (vs', es'') := split_vals es' in
+    ((val__CONST t v) :: vs', es'')
+  | _ => ([::], es)
+  end.
+
+Lemma split_vals_inverse : forall vs es es',
+  split_vals es = (vs, es') ->
+  es = list__val__admininstr vs ++ es'.
+Proof.
+  move => vs es es' H.
+  move: vs es' H.
+  elim: es => [ | e es' IH].
+  - move => vs es' H.
+    case: H => Hvs Hes'.
+    by rewrite -Hvs -Hes'.
+  - (* TODO: Using case tactic involves introducing constructor parameters of e
+             which is tedious *)
+    destruct e;
+    try (move => vs es'' H;
+         case: H => Hvs Hes'';
+         by rewrite -Hvs -Hes'').
+    move => vs es'' H.
+    case Ees': (split_vals es') => [svs ses].
+    rewrite /= Ees' in H.
+    case: H => Hvs Hes''.
+    move/IH: Ees' => {}IH.
+    by rewrite -Hvs -Hes'' IH /=.
+Qed.
+
+Lemma split_vals_prefix : forall vs e es,
+  (forall t v, e <> admininstr__CONST t v) ->
+  split_vals (list__val__admininstr vs ++ [:: e] ++ es) = (vs, [:: e] ++ es).
+Proof.
+  move => vs e es H.
+  elim: vs => [| v vs'].
+  - case: e H => //=.
+    move => t' v' Hcontra.
+    by move/(_ t' v'): Hcontra.
+  - case: v => /=.
+    move => t' v' IH.
+    by rewrite IH.
+Qed.
+
+Lemma br_reduce_decidable : forall es,
+  decidable (br_reduce es).
+Proof.
+  rewrite /decidable /br_reduce.
+  move => es.
+  case Ees: (split_vals es) => [vs es'].
+  case Ees': es' => [| e es''].
+  - right. move => [vcs [l [es''' Hcontra]]].
+    rewrite Hcontra in Ees.
+    rewrite (split_vals_prefix vcs (admininstr__BR l) es''') in Ees; last by [].
+    case: Ees => Hvs Hes'.
+    by rewrite Ees' in Hes'.
+  - (* TODO: Using case tactic involves introducing constructor parameters of e
+             which is tedious *)
+    destruct e;
+    try (right;
+         move => [vcs [l [es''' Hcontra]]];
+         rewrite Hcontra in Ees;
+         rewrite (split_vals_prefix vcs (admininstr__BR l) es''') in Ees; last by [];
+         case: Ees => Hvs Hes';
+         by rewrite Ees' in Hes').
+    left. exists vs, v_labelidx, es''.
+    rewrite /= -Ees'.
+    by rewrite (split_vals_inverse _ _ _ Ees).
+Qed.
+
+Lemma not_br_reduce_not_lf_br : forall es,
+  ~ (br_reduce es) -> not_lf_br es.
+Proof.
+  rewrite /br_reduce /not_lf_br.
+  move => es H1 vcs l es' H2.
+  apply: H1. by exists vcs, l, es'. 
+Qed.
+
+Lemma not_return_reduce_not_lf_return : forall es,
+  ~ (return_reduce es) -> not_lf_return es.
+Proof.
+  rewrite /return_reduce /not_lf_return.
+  move => es H1 vcs es' H2.
+  apply: H1. by exists vcs, es'.
+Qed.
+
+Lemma not_lf_br_singleton : forall e l,
+  not_lf_br [:: e] -> e <> admininstr__BR l.
+Proof.
+  move => e l H Hcontra.
+  rewrite Hcontra /not_lf_br in H.
+  by move/(_ [::] l [::]): H => H.
+Qed.
+
+Lemma not_fl_return_singleton : forall e,
+  not_lf_return [:: e] -> e <> admininstr__RETURN.
+Proof.
+  move => e H Hcontra.
+  rewrite Hcontra /not_lf_return in H.
+  by move/(_ [::] [::]): H => H.
+Qed.
+
+(*
+Definition not_lf_br es := Forall (fun e => forall l, e <> admininstr__BR l) es.
+
+Definition not_lf_return es := Forall (fun e => e <> admininstr__RETURN) es.
+
+Lemma cat_eq_nil : forall A (l1 l2 : seq A),
+  (l1 ++ l2) = [::] -> l1 = [::] /\ l2 = [::].
+Proof.
+  move => A l1 l2.
+  by case: l1; case l2.
+Qed.
+
+Lemma Forall_cat : forall A (P : A -> Prop) (l1 l2 : seq A),
+  Forall P (l1 ++ l2) <-> Forall P l1 /\ Forall P l2.
+Proof.
+  move => A P l1 l2. split.
+  - elim: l1 => [|x' l1'] //=.
+    move => IH Hl. inversion Hl.
+    move/IH: H2 => [Hl1' Hl2].
+    split => //=.
+    by apply: Forall_cons => //=.
+  - move => [F1 F2].
+    elim: F1 => [|x l Px Fl IH] //=.
+    by apply: Forall_cons.
+Qed.
+
+Lemma not_lf_br_cat : forall es1 es2,
+  not_lf_br (es1 ++ es2) <-> not_lf_br es1 /\ not_lf_br es2.
+Proof.
+  rewrite /not_lf_br.
+  by apply: Forall_cat.
+Qed.
+
+Lemma not_lf_return_cat : forall es1 es2,
+  not_lf_return (es1 ++ es2) <-> not_lf_return es1 /\ not_lf_return es2.
+Proof.
+  rewrite /not_lf_return.
+  by apply: Forall_cat.
+Qed. *)
+
 (* MEMO: be_typing -> Instrs_ok *)
 (* MEMO: f.(f_inst) -> f.(frame__MODULE) *)
 (* TODO: Reorder premises in consistent order *)
@@ -449,8 +612,8 @@ Lemma t_progress_be: forall s C C' f vcs bes tf ts1 ts2 lab ret,
   Module_instance_ok s f.(frame__MODULE) C' ->
   map typeof vcs = ts1 ->
   Store_ok s ->
-  (* not_lf_br (list__instr__admininstr bes) -> *)
-  (* not_lf_return (list__instr__admininstr bes) -> *)
+  not_lf_br (list__instr__admininstr bes) ->
+  not_lf_return (list__instr__admininstr bes) ->
   const_list (list__instr__admininstr bes) \/
   exists s' f' es', Step (config__ (state__ s f) (list__val__admininstr vcs ++ list__instr__admininstr bes)) (config__ (state__ s' f') es').
 Proof.
@@ -464,8 +627,8 @@ Proof.
       Module_instance_ok s f.(frame__MODULE) C' ->
       map typeof vcs = ts1 ->
       Store_ok s ->
-      (* not_lf_br (list__instr__admininstr [:: be]) -> *)
-      (* not_lf_return (list__instr__admininstr [:: be]) -> *)
+      not_lf_br (list__instr__admininstr [:: be]) ->
+      not_lf_return (list__instr__admininstr [:: be]) ->
       const_list (list__instr__admininstr [:: be]) \/
       exists s' f' es', Step (config__ (state__ s f) (list__val__admininstr vcs ++ list__instr__admininstr [:: be])) (config__ (state__ s' f') es'))
     (P0 := fun C bes tf (Hinstrs : Instrs_ok C bes tf) =>
@@ -475,596 +638,613 @@ Proof.
       Module_instance_ok s f.(frame__MODULE) C' ->
       map typeof vcs = ts1 ->
       Store_ok s ->
-      (* not_lf_br (list__instr__admininstr bes) -> *)
-      (* not_lf_return (list__instr__admininstr bes) -> *)
+      not_lf_br (list__instr__admininstr bes) ->
+      not_lf_return (list__instr__admininstr bes) ->
       const_list (list__instr__admininstr bes) \/
       exists s' f' es', Step (config__ (state__ s f) (list__val__admininstr vcs ++ list__instr__admininstr bes)) (config__ (state__ s' f') es'))
       => // {C bes tf Hinstrs}.
-    - (* Instr_ok__nop *)
-      move => C.
-      move => s f C' vcs ts1 ts2 lab ret Htf Hcontext Hmod Hts Hstore.
-      (* TODO: Can we get rid of ++ [::] in exists? *)
-      right. exists s, f, (list__val__admininstr vcs ++ [::] ++ [::]).
-      apply Step__ctxt_seq with
-        (v_admininstr := [:: admininstr__NOP]).
-      by apply: Step__pure Step_pure__nop.
-    - (* Instr_ok__unreachable *)
-      move => C ts1 ts2.
-      move => s f C' vcs ts1' ts2' lab ret Htf Hcontext Hmod Hts Hstore.
-      (* TODO: Can we get rid of ++ [::] in exists? *)
-      right. exists s, f, (list__val__admininstr vcs ++ [:: admininstr__TRAP] ++ [::]).
-      apply Step__ctxt_seq with
-        (v_admininstr := [:: admininstr__UNREACHABLE]).
-      by apply: Step__pure Step_pure__unreachable.
-    - (* Instr_ok__drop *)
-      move => C t.
-      move => s f C' vcs ts1' ts2' lab ret Htf Hcontext Hmod Hts Hstore.
-      right.
-      (* TODO: Replace injection in other places with case
-               e.g. injection Htf => _ Htf1. rewrite -{}Htf1 in Hts. *)
-      (* TODO: Use invert_typeof_vcs in t_progress_e too. *)
-      case: Htf => Htf1 _. rewrite -Htf1 in Hts. invert_typeof_vcs.
-      exists s, f, [::].
+  - (* Instr_ok__nop *)
+    move => C.
+    move => s f C' vcs ts1 ts2 lab ret Htf Hcontext Hmod Hts Hstore Hnotbr Hnotret.
+    (* TODO: Can we get rid of ++ [::] in exists? *)
+    right. exists s, f, (list__val__admininstr vcs ++ [::] ++ [::]).
+    apply Step__ctxt_seq with
+      (v_admininstr := [:: admininstr__NOP]).
+    by apply: Step__pure Step_pure__nop.
+  - (* Instr_ok__unreachable *)
+    move => C ts1 ts2.
+    move => s f C' vcs ts1' ts2' lab ret Htf Hcontext Hmod Hts Hstore Hnotbr Hnotret.
+    (* TODO: Can we get rid of ++ [::] in exists? *)
+    right. exists s, f, (list__val__admininstr vcs ++ [:: admininstr__TRAP] ++ [::]).
+    apply Step__ctxt_seq with
+      (v_admininstr := [:: admininstr__UNREACHABLE]).
+    by apply: Step__pure Step_pure__unreachable.
+  - (* Instr_ok__drop *)
+    move => C t.
+    move => s f C' vcs ts1' ts2' lab ret Htf Hcontext Hmod Hts Hstore Hnotbr Hnotret.
+    right.
+    (* TODO: Replace injection in other places with case
+              e.g. injection Htf => _ Htf1. rewrite -{}Htf1 in Hts. *)
+    (* TODO: Use invert_typeof_vcs in t_progress_e too. *)
+    case: Htf => Htf1 _. rewrite -Htf1 in Hts. invert_typeof_vcs.
+    exists s, f, [::].
+    apply: Step__pure.
+    by apply: Step_pure__drop.
+  - (* Instr_ok__select *)
+    move => C t.
+    move => s f C' vcs ts1' ts2' lab ret Htf Hcontext Hmod Hts Hstore Hnotbr Hnotret.
+    right.
+    case: Htf => Htf1 _. rewrite -Htf1 in Hts. invert_typeof_vcs.
+    invert_val_wf v3. rewrite /= in Ht3. rewrite Ht3.
+    case: v3 => [| v3'].
+    - exists s, f, (list__val__admininstr [:: v2]).
       apply: Step__pure.
-      by apply: Step_pure__drop.
-    - (* Instr_ok__select *)
-      move => C t.
-      move => s f C' vcs ts1' ts2' lab ret Htf Hcontext Hmod Hts Hstore.
-      right.
-      case: Htf => Htf1 _. rewrite -Htf1 in Hts. invert_typeof_vcs.
-      invert_val_wf v3. rewrite /= in Ht3. rewrite Ht3.
-      case: v3 => [| v3'].
-      - exists s, f, (list__val__admininstr [:: v2]).
-        apply: Step__pure.
-        by apply: Step_pure__select_false.
-      - exists s, f, (list__val__admininstr [:: v1]).
-        apply: Step__pure.
-        by apply: Step_pure__select_true.
-    - (* Instr_ok__block *)
-      move => C bt bes _ _.
-      move => s f C' vcs ts1 ts2 lab ret Htf Hcontext Hmod Hts Hstore.
-      right. exists s, f, [:: admininstr__LABEL_ (fun_optionSize bt) [::] (list__instr__admininstr bes)].
-      case: Htf => Htf1 _. rewrite -Htf1 in Hts. invert_typeof_vcs.
-      apply: Step__read. apply: Step_read__block.
-      case: bt => [bt |] //=; by [right | left].
-    - (* Instr_ok__loop *)
-      move => C bt bes _ _.
-      move => s f C' vcs ts1 ts2 lab ret Htf Hcontext Hmod Hts Hstore.
-      right. exists s, f, [:: admininstr__LABEL_ (fun_optionSize bt) [:: instr__LOOP bt bes] (list__instr__admininstr bes)].
-      case: Htf => Htf1 _. rewrite -Htf1 in Hts. invert_typeof_vcs.
-      apply: Step__read. apply: Step_read__loop.
-      case: bt => [bt |] //=; by [right | left].
-    - (* Instr_ok__if *)
-      move => C bt bes1 bes2 _ _ _ _.
-      move => s f C' vcs ts1 ts2 lab ret Htf Hcontext Hmod Hts Hstore.
-      right.
-      case: Htf => Htf1 _. rewrite -Htf1 in Hts. invert_typeof_vcs.
-      invert_val_wf v1. rewrite /= in Ht1. rewrite Ht1.
-      case: v1 => [| v1'].
-      - exists s, f, [:: admininstr__BLOCK bt bes2].
-        apply: Step__pure.
-        by apply: Step_pure__if_false.
-      - exists s, f, [:: admininstr__BLOCK bt bes1].
-        apply: Step__pure.
-        by apply: Step_pure__if_true.
-    - (* Instr_ok__br *)
-      (* TODO: This case should be discarded by not_lf_br *)
-      by admit.
-    - (* Instr_ok__br_if *)
-      move => C l ts Hlen Hlookup.
-      move => s f C' vcs ts1 ts2 lab ret Htf Hcontext Hmod Hts Hstore.
-      right.
-      case: Htf => Htf1 _. rewrite -{}Htf1 in Hts.
-      move/typeof_append: Hts => [v1 [Hvcs [Hts Ht1]]]. rewrite {}Hvcs.
-      set vcs' := take (size (option_to_list ts)) vcs.
-      invert_val_wf v1. rewrite /= in Ht1. rewrite Ht1.
-      case: v1 => [| v1'].
-      + exists s, f, (list__val__admininstr vcs').
-        (* TODO: Can we get rid of these rewrites? *)
-        have -> : forall vcs1 vcs2, list__val__admininstr (vcs1 ++ vcs2) = list__val__admininstr vcs1 ++ list__val__admininstr vcs2.
-        { move => vcs1 vcs2. rewrite /list__val__admininstr. rewrite !map_map. by rewrite map_cat. }
-        have -> : (list__val__admininstr vcs' ++ list__val__admininstr [:: val__CONST (valtype__INN inn__I32) (val___inn__entry 0)]) ++ [:: admininstr__BR_IF l] = list__val__admininstr vcs' ++ (list__val__admininstr [:: val__CONST (valtype__INN inn__I32) (val___inn__entry 0)] ++ [:: admininstr__BR_IF l]) ++ [::]. { by rewrite -2!catA cats0. }
-        have {2}-> : list__val__admininstr vcs' = list__val__admininstr vcs' ++ [::] ++ [::]. { by rewrite 2!cats0. }
-        (* TODO: This fails while vanilla tactic succeeds *)
-        (* apply: Step__ctxt_seq. *)
-        apply Step__ctxt_seq.
-        apply: Step__pure.
-        by apply: Step_pure__br_if_false.
-      + exists s, f, (list__val__admininstr vcs' ++ [:: admininstr__BR l]).
-        (* TODO: Can we get rid of these rewrites? *)
-        have -> : forall vcs1 vcs2, list__val__admininstr (vcs1 ++ vcs2) = list__val__admininstr vcs1 ++ list__val__admininstr vcs2.
-        { move => vcs1 vcs2. rewrite /list__val__admininstr. rewrite !map_map. by rewrite map_cat. }
-        have -> : (list__val__admininstr vcs' ++ list__val__admininstr [:: val__CONST (valtype__INN inn__I32) (val___inn__entry v1'.+1)]) ++ [:: admininstr__BR_IF l] = list__val__admininstr vcs' ++ (list__val__admininstr [:: val__CONST (valtype__INN inn__I32) (val___inn__entry v1'.+1)] ++ [:: admininstr__BR_IF l]) ++ [::]. { by rewrite -2!catA cats0. }
-        have -> : list__val__admininstr vcs' ++ [:: admininstr__BR l] = list__val__admininstr vcs' ++ [:: admininstr__BR l] ++ [::]. { by rewrite !cats0. }
-        (* TODO: This fails while vanilla tactic succeeds *)
-        (* apply: Step__ctxt_seq. *)
-        apply Step__ctxt_seq.
-        apply: Step__pure.
-        by apply: Step_pure__br_if_true.
-    - (* Instr_ok__br_table *)
-      move => C ls lN ts1 ts ts2 HlenlN Hlenls HlookuplN Hlookupls.
-      move => s f C' vcs ts1' ts2' lab ret Htf Hcontext Hmod Hts Hstore.
-      right.
-      case: Htf => Htf1 _. rewrite -{}Htf1 in Hts.
-      rewrite cat_app catA in Hts.
-      move/typeof_append: Hts => [v1 [Hvcs [Hts Ht1]]]. rewrite {}Hvcs.
-      set vcs' := take (size (ts1 ++ option_to_list ts)) vcs.
-      invert_val_wf v1. rewrite /= in Ht1. rewrite Ht1.
-      case Hv1: (v1 < size ls);
-      move/ltP: Hv1 => Hv1.
-      + exists s, f, (list__val__admininstr vcs' ++ [:: admininstr__BR (lookup_total ls v1)]).
-        (* TODO: Can we get rid of these rewrites? *)
-        have -> : forall vcs1 vcs2, list__val__admininstr (vcs1 ++ vcs2) = list__val__admininstr vcs1 ++ list__val__admininstr vcs2.
-        { move => vcs1 vcs2. rewrite /list__val__admininstr. rewrite !map_map. by rewrite map_cat. }
-        rewrite -catA.
-        have -> : forall es1 es2 es3, es1 ++ es2 ++ es3 = es1 ++ (es2 ++ es3) ++ [::]. { move => T es1 es2 es3. by rewrite -catA cats0. }
-        have -> : list__val__admininstr vcs' ++ [:: admininstr__BR (lookup_total ls v1)] = list__val__admininstr vcs' ++ [:: admininstr__BR (lookup_total ls v1)] ++ [::]. { by rewrite !cats0. }
-        (* TODO: This fails while vanilla tactic succeeds *)
-        (* apply: Step__ctxt_seq. *)
-        apply Step__ctxt_seq.
-        apply: Step__pure.
-        apply: Step_pure__br_table_lt.
-        by rewrite length_size.
-      + exists s, f, (list__val__admininstr vcs' ++ [:: admininstr__BR lN]).
-        (* TODO: Can we get rid of these rewrites? *)
-        have -> : forall vcs1 vcs2, list__val__admininstr (vcs1 ++ vcs2) = list__val__admininstr vcs1 ++ list__val__admininstr vcs2.
-        { move => vcs1 vcs2. rewrite /list__val__admininstr. rewrite !map_map. by rewrite map_cat. }
-        rewrite -catA.
-        have -> : forall es1 es2 es3, es1 ++ es2 ++ es3 = es1 ++ (es2 ++ es3) ++ [::]. { move => T es1 es2 es3. by rewrite -catA cats0. }
-        have -> : list__val__admininstr vcs' ++ [:: admininstr__BR lN] = list__val__admininstr vcs' ++ [:: admininstr__BR lN] ++ [::]. { by rewrite !cats0. }
-        (* TODO: This fails while vanilla tactic succeeds *)
-        (* apply: Step__ctxt_seq. *)
-        apply Step__ctxt_seq.
-        apply: Step__pure.
-        apply: Step_pure__br_table_ge.
-        rewrite length_size.
-        move/ltP: Hv1 => Hv1. apply/leP.
-        by rewrite /ge leqNgt.
-    - (* Instr_ok__call *)
-      move => C x ts1 ts2 Haddr Hlookup.
-      move => s f C' vcs ts1' ts2' lab ret Htf Hcontext Hmod Hts Hstore.
-      (* TODO: Can we get rid of ++ [::] in exists? *)
-      right. exists s, f, (list__val__admininstr vcs ++ [:: admininstr__CALL_ADDR (lookup_total (fun_funcaddr (state__ s f)) x)] ++ [::]).
+      by apply: Step_pure__select_false.
+    - exists s, f, (list__val__admininstr [:: v1]).
+      apply: Step__pure.
+      by apply: Step_pure__select_true.
+  - (* Instr_ok__block *)
+    move => C bt bes _ _.
+    move => s f C' vcs ts1 ts2 lab ret Htf Hcontext Hmod Hts Hstore Hnotbr Hnotret.
+    right. exists s, f, [:: admininstr__LABEL_ (fun_optionSize bt) [::] (list__instr__admininstr bes)].
+    case: Htf => Htf1 _. rewrite -Htf1 in Hts. invert_typeof_vcs.
+    apply: Step__read. apply: Step_read__block.
+    case: bt Hnotbr Hnotret => [bt |] Hnotbr Hnotret //=; by [right | left].
+  - (* Instr_ok__loop *)
+    move => C bt bes _ _.
+    move => s f C' vcs ts1 ts2 lab ret Htf Hcontext Hmod Hts Hstore Hnotbr Hnotret.
+    right. exists s, f, [:: admininstr__LABEL_ (fun_optionSize bt) [:: instr__LOOP bt bes] (list__instr__admininstr bes)].
+    case: Htf => Htf1 _. rewrite -Htf1 in Hts. invert_typeof_vcs.
+    apply: Step__read. apply: Step_read__loop.
+    case: bt Hnotbr Hnotret => [bt |] Hnotbr Hnotret //=; by [right | left].
+  - (* Instr_ok__if *)
+    move => C bt bes1 bes2 _ _ _ _.
+    move => s f C' vcs ts1 ts2 lab ret Htf Hcontext Hmod Hts Hstore Hnotbr Hnotret.
+    right.
+    case: Htf => Htf1 _. rewrite -Htf1 in Hts. invert_typeof_vcs.
+    invert_val_wf v1. rewrite /= in Ht1. rewrite Ht1.
+    case: v1 => [| v1'].
+    - exists s, f, [:: admininstr__BLOCK bt bes2].
+      apply: Step__pure.
+      by apply: Step_pure__if_false.
+    - exists s, f, [:: admininstr__BLOCK bt bes1].
+      apply: Step__pure.
+      by apply: Step_pure__if_true.
+  - (* Instr_ok__br *)
+    move => C l ts1 ts ts2 Hlablen Hlablookup.
+    move => s f C' vcs ts1' ts2' lab ret Htf Hcontext Hmod Hts Hstore Hnotbr Hnotret.
+    rewrite /not_lf_br /= in Hnotbr.
+    inversion Hnotbr as [|? ? Hcontra].
+    by move/(_ l): Hcontra.
+  - (* Instr_ok__br_if *)
+    move => C l ts Hlen Hlookup.
+    move => s f C' vcs ts1 ts2 lab ret Htf Hcontext Hmod Hts Hstore Hnotbr Hnotret.
+    right.
+    case: Htf => Htf1 _. rewrite -{}Htf1 in Hts.
+    move/typeof_append: Hts => [v1 [Hvcs [Hts Ht1]]]. rewrite {}Hvcs.
+    set vcs' := take (size (option_to_list ts)) vcs.
+    invert_val_wf v1. rewrite /= in Ht1. rewrite Ht1.
+    case: v1 => [| v1'].
+    + exists s, f, (list__val__admininstr vcs').
       (* TODO: Can we get rid of these rewrites? *)
-      rewrite -[list__val__admininstr vcs ++ _]cats0 -catA.
+      have -> : forall vcs1 vcs2, list__val__admininstr (vcs1 ++ vcs2) = list__val__admininstr vcs1 ++ list__val__admininstr vcs2.
+      { move => vcs1 vcs2. rewrite /list__val__admininstr. rewrite !map_map. by rewrite map_cat. }
+      have -> : (list__val__admininstr vcs' ++ list__val__admininstr [:: val__CONST (valtype__INN inn__I32) (val___inn__entry 0)]) ++ [:: admininstr__BR_IF l] = list__val__admininstr vcs' ++ (list__val__admininstr [:: val__CONST (valtype__INN inn__I32) (val___inn__entry 0)] ++ [:: admininstr__BR_IF l]) ++ [::]. { by rewrite -2!catA cats0. }
+      have {2}-> : list__val__admininstr vcs' = list__val__admininstr vcs' ++ [::] ++ [::]. { by rewrite 2!cats0. }
+      (* TODO: This fails while vanilla tactic succeeds *)
+      (* apply: Step__ctxt_seq. *)
+      apply Step__ctxt_seq.
+      apply: Step__pure.
+      by apply: Step_pure__br_if_false.
+    + exists s, f, (list__val__admininstr vcs' ++ [:: admininstr__BR l]).
+      (* TODO: Can we get rid of these rewrites? *)
+      have -> : forall vcs1 vcs2, list__val__admininstr (vcs1 ++ vcs2) = list__val__admininstr vcs1 ++ list__val__admininstr vcs2.
+      { move => vcs1 vcs2. rewrite /list__val__admininstr. rewrite !map_map. by rewrite map_cat. }
+      have -> : (list__val__admininstr vcs' ++ list__val__admininstr [:: val__CONST (valtype__INN inn__I32) (val___inn__entry v1'.+1)]) ++ [:: admininstr__BR_IF l] = list__val__admininstr vcs' ++ (list__val__admininstr [:: val__CONST (valtype__INN inn__I32) (val___inn__entry v1'.+1)] ++ [:: admininstr__BR_IF l]) ++ [::]. { by rewrite -2!catA cats0. }
+      have -> : list__val__admininstr vcs' ++ [:: admininstr__BR l] = list__val__admininstr vcs' ++ [:: admininstr__BR l] ++ [::]. { by rewrite !cats0. }
+      (* TODO: This fails while vanilla tactic succeeds *)
+      (* apply: Step__ctxt_seq. *)
+      apply Step__ctxt_seq.
+      apply: Step__pure.
+      by apply: Step_pure__br_if_true.
+  - (* Instr_ok__br_table *)
+    move => C ls lN ts1 ts ts2 HlenlN Hlenls HlookuplN Hlookupls.
+    move => s f C' vcs ts1' ts2' lab ret Htf Hcontext Hmod Hts Hstore Hnotbr Hnotret.
+    right.
+    case: Htf => Htf1 _. rewrite -{}Htf1 in Hts.
+    rewrite cat_app catA in Hts.
+    move/typeof_append: Hts => [v1 [Hvcs [Hts Ht1]]]. rewrite {}Hvcs.
+    set vcs' := take (size (ts1 ++ option_to_list ts)) vcs.
+    invert_val_wf v1. rewrite /= in Ht1. rewrite Ht1.
+    case Hv1: (v1 < size ls);
+    move/ltP: Hv1 => Hv1.
+    + exists s, f, (list__val__admininstr vcs' ++ [:: admininstr__BR (lookup_total ls v1)]).
+      (* TODO: Can we get rid of these rewrites? *)
+      have -> : forall vcs1 vcs2, list__val__admininstr (vcs1 ++ vcs2) = list__val__admininstr vcs1 ++ list__val__admininstr vcs2.
+      { move => vcs1 vcs2. rewrite /list__val__admininstr. rewrite !map_map. by rewrite map_cat. }
+      rewrite -catA.
+      have -> : forall es1 es2 es3, es1 ++ es2 ++ es3 = es1 ++ (es2 ++ es3) ++ [::]. { move => T es1 es2 es3. by rewrite -catA cats0. }
+      have -> : list__val__admininstr vcs' ++ [:: admininstr__BR (lookup_total ls v1)] = list__val__admininstr vcs' ++ [:: admininstr__BR (lookup_total ls v1)] ++ [::]. { by rewrite !cats0. }
+      (* TODO: This fails while vanilla tactic succeeds *)
+      (* apply: Step__ctxt_seq. *)
+      apply Step__ctxt_seq.
+      apply: Step__pure.
+      apply: Step_pure__br_table_lt.
+      by rewrite length_size.
+    + exists s, f, (list__val__admininstr vcs' ++ [:: admininstr__BR lN]).
+      (* TODO: Can we get rid of these rewrites? *)
+      have -> : forall vcs1 vcs2, list__val__admininstr (vcs1 ++ vcs2) = list__val__admininstr vcs1 ++ list__val__admininstr vcs2.
+      { move => vcs1 vcs2. rewrite /list__val__admininstr. rewrite !map_map. by rewrite map_cat. }
+      rewrite -catA.
+      have -> : forall es1 es2 es3, es1 ++ es2 ++ es3 = es1 ++ (es2 ++ es3) ++ [::]. { move => T es1 es2 es3. by rewrite -catA cats0. }
+      have -> : list__val__admininstr vcs' ++ [:: admininstr__BR lN] = list__val__admininstr vcs' ++ [:: admininstr__BR lN] ++ [::]. { by rewrite !cats0. }
+      (* TODO: This fails while vanilla tactic succeeds *)
+      (* apply: Step__ctxt_seq. *)
+      apply Step__ctxt_seq.
+      apply: Step__pure.
+      apply: Step_pure__br_table_ge.
+      rewrite length_size.
+      move/ltP: Hv1 => Hv1. apply/leP.
+      by rewrite /ge leqNgt.
+  - (* Instr_ok__call *)
+    move => C x ts1 ts2 Haddr Hlookup.
+    move => s f C' vcs ts1' ts2' lab ret Htf Hcontext Hmod Hts Hstore Hnotbr Hnotret.
+    (* TODO: Can we get rid of ++ [::] in exists? *)
+    right. exists s, f, (list__val__admininstr vcs ++ [:: admininstr__CALL_ADDR (lookup_total (fun_funcaddr (state__ s f)) x)] ++ [::]).
+    (* TODO: Can we get rid of these rewrites? *)
+    rewrite -[list__val__admininstr vcs ++ _]cats0 -catA.
+    apply Step__ctxt_seq with
+      (v_admininstr := [:: admininstr__CALL x]).
+    apply: Step__read. apply: Step_read__call.
+    rewrite !length_size in Haddr *.
+    (* TODO: Extract this into a separate lemma *)
+    have H1 : context__FUNCS C = context__FUNCS C'.
+    { move => {Haddr Hlookup}.
+      case: C Hcontext => ? ? ? ? ? ? ? ? Hcontext.
+      case: C' Hcontext Hmod => ? ? ? ? ? ? ? ? Hcontext Hmod.
+      inversion Hmod => /=. inversion Hcontext => /=. by []. }
+    rewrite {}H1 in Haddr.
+    (* TODO: Extract this into a separate lemma *)
+    have H2 : size (context__FUNCS C') = size (fun_funcaddr (state__ s f)).
+    { move => {Hcontext Haddr}.
+      case: C' Hmod => ? ? ? ? ? ? ? ? Hmod.
+      inversion Hmod as [? ? ? ? ? ? ? ? ? ? ? ? ? ? ? ? ? ? ? ? ? Hs Hf] => //=.
+      by rewrite -Hf => //=. }
+    by rewrite -{}H2.
+  - (* Instr_ok__call_indirect *)
+    move => C x ts1 ts2 Haddr Hlookup.
+    move => s f C' vcs ts1' ts2' lab ret Htf Hcontext Hmod Hts Hstore Hnotbr Hnotret.
+    right.
+    (* TODO: Make use of typeof_append in t_progress_e too *)
+    case: Htf => Htf1 _. rewrite -{}Htf1 in Hts.
+    move/typeof_append: Hts => [v1 [Hvcs [Hts Ht1]]]. rewrite {}Hvcs.
+    invert_val_wf v1. rewrite /= in Ht1. rewrite Ht1.
+    case E1: (lookup_total (tableinst__REFS (fun_table (state__ s f) 0)) v1) => [a |].
+    case E2: (fun_type (state__ s f) x == funcinst__TYPE (lookup_total (fun_funcinst (state__ s f)) a)).
+    case E3: (v1 < Datatypes.length (tableinst__REFS (fun_table (state__ s f) 0))).
+    case E4: (a < Datatypes.length (store__FUNCS s)).
+    all: try move/eqP: E2 => E2;
+          try move/ltP: E3 => E3;
+          try move/ltP: E4 => E4.
+    + exists s, f, (list__val__admininstr (take (size ts1) vcs) ++ [:: admininstr__CALL_ADDR a]).
+      (* TODO: Can we get rid of these rewrites? *)
+      have -> : (list__val__admininstr (take (size ts1) vcs ++ [:: val__CONST (valtype__INN inn__I32) (val___inn__entry v1)]) ++ [:: admininstr__CALL_INDIRECT x]) = (list__val__admininstr (take (size ts1) vcs) ++ (list__val__admininstr [:: val__CONST (valtype__INN inn__I32) (val___inn__entry v1)] ++ [:: admininstr__CALL_INDIRECT x]) ++ [::]).
+      { rewrite cats0 catA. rewrite /list__val__admininstr. rewrite !map_map. rewrite map_cat. by []. }
+      rewrite -[[:: admininstr__CALL_ADDR a]]cats0.
       apply Step__ctxt_seq with
-        (v_admininstr := [:: admininstr__CALL x]).
-      apply: Step__read. apply: Step_read__call.
-      rewrite !length_size in Haddr *.
-      (* TODO: Extract this into a separate lemma *)
-      have H1 : context__FUNCS C = context__FUNCS C'.
-      { move => {Haddr Hlookup}.
-        case: C Hcontext => ? ? ? ? ? ? ? ? Hcontext.
-        case: C' Hcontext Hmod => ? ? ? ? ? ? ? ? Hcontext Hmod.
-        inversion Hmod => /=. inversion Hcontext => /=. by []. }
-      rewrite {}H1 in Haddr.
-      (* TODO: Extract this into a separate lemma *)
-      have H2 : size (context__FUNCS C') = size (fun_funcaddr (state__ s f)).
-      { move => {Hcontext Haddr}.
-        case: C' Hmod => ? ? ? ? ? ? ? ? Hmod.
-        inversion Hmod as [? ? ? ? ? ? ? ? ? ? ? ? ? ? ? ? ? ? ? ? ? Hs Hf] => //=.
-        by rewrite -Hf => //=. }
-      by rewrite -{}H2.
-    - (* Instr_ok__call_indirect *)
-      move => C x ts1 ts2 Haddr Hlookup.
-      move => s f C' vcs ts1' ts2' lab ret Htf Hcontext Hmod Hts Hstore.
-      right.
-      (* TODO: Make use of typeof_append in t_progress_e too *)
-      case: Htf => Htf1 _. rewrite -{}Htf1 in Hts.
-      move/typeof_append: Hts => [v1 [Hvcs [Hts Ht1]]]. rewrite {}Hvcs.
-      invert_val_wf v1. rewrite /= in Ht1. rewrite Ht1.
-      case E1: (lookup_total (tableinst__REFS (fun_table (state__ s f) 0)) v1) => [a |].
-      case E2: (fun_type (state__ s f) x == funcinst__TYPE (lookup_total (fun_funcinst (state__ s f)) a)).
-      case E3: (v1 < Datatypes.length (tableinst__REFS (fun_table (state__ s f) 0))).
-      case E4: (a < Datatypes.length (store__FUNCS s)).
-      all: try move/eqP: E2 => E2;
-           try move/ltP: E3 => E3;
-           try move/ltP: E4 => E4.
-      + exists s, f, (list__val__admininstr (take (size ts1) vcs) ++ [:: admininstr__CALL_ADDR a]).
-        (* TODO: Can we get rid of these rewrites? *)
-        have -> : (list__val__admininstr (take (size ts1) vcs ++ [:: val__CONST (valtype__INN inn__I32) (val___inn__entry v1)]) ++ [:: admininstr__CALL_INDIRECT x]) = (list__val__admininstr (take (size ts1) vcs) ++ (list__val__admininstr [:: val__CONST (valtype__INN inn__I32) (val___inn__entry v1)] ++ [:: admininstr__CALL_INDIRECT x]) ++ [::]).
-        { rewrite cats0 catA. rewrite /list__val__admininstr. rewrite !map_map. rewrite map_cat. by []. }
-        rewrite -[[:: admininstr__CALL_ADDR a]]cats0.
-        apply Step__ctxt_seq with
-          (v_admininstr := list__val__admininstr [:: val__CONST (valtype__INN inn__I32) (val___inn__entry v1)] ++ [:: admininstr__CALL_INDIRECT x]%list).
-        apply: Step__read.
-        apply: Step_read__call_indirect_call => //=.
-      + exists s, f, (list__val__admininstr (take (size ts1) vcs) ++ [:: admininstr__TRAP]).
-        (* TODO: Can we get rid of these rewrites? *)
-        have -> : (list__val__admininstr (take (size ts1) vcs ++ [:: val__CONST (valtype__INN inn__I32) (val___inn__entry v1)]) ++ [:: admininstr__CALL_INDIRECT x]) = (list__val__admininstr (take (size ts1) vcs) ++ (list__val__admininstr [:: val__CONST (valtype__INN inn__I32) (val___inn__entry v1)] ++ [:: admininstr__CALL_INDIRECT x]) ++ [::]).
-        { rewrite cats0 catA. rewrite /list__val__admininstr. rewrite !map_map. rewrite map_cat. by []. }
-        rewrite -[[:: admininstr__TRAP]]cats0.
-        apply Step__ctxt_seq with
-          (v_admininstr := list__val__admininstr [:: val__CONST (valtype__INN inn__I32) (val___inn__entry v1)] ++ [:: admininstr__CALL_INDIRECT x]).
-        apply: Step__read.
-        apply: Step_read__call_indirect_trap.
-        move => Hcontra.
-        inversion Hcontra as [[s' f'] i' x' a' E3' E4' E1' E2' [Hs' Hf' Hi' Hx']].
-        rewrite E1 in E1'. inversion E1' as [E1''].
-        rewrite -E1'' in E4'.
-        by move/E4: E4' => E4''.
-      + exists s, f, (list__val__admininstr (take (size ts1) vcs) ++ [:: admininstr__TRAP]).
-        (* TODO: Can we get rid of these rewrites? *)
-        have -> : (list__val__admininstr (take (size ts1) vcs ++ [:: val__CONST (valtype__INN inn__I32) (val___inn__entry v1)]) ++ [:: admininstr__CALL_INDIRECT x]) = (list__val__admininstr (take (size ts1) vcs) ++ (list__val__admininstr [:: val__CONST (valtype__INN inn__I32) (val___inn__entry v1)] ++ [:: admininstr__CALL_INDIRECT x]) ++ [::]).
-        { rewrite cats0 catA. rewrite /list__val__admininstr. rewrite !map_map. rewrite map_cat. by []. }
-        rewrite -[[:: admininstr__TRAP]]cats0.
-        apply Step__ctxt_seq with
-          (v_admininstr := list__val__admininstr [:: val__CONST (valtype__INN inn__I32) (val___inn__entry v1)] ++ [:: admininstr__CALL_INDIRECT x]).
-        apply: Step__read.
-        apply: Step_read__call_indirect_trap.
-        move => Hcontra.
-        inversion Hcontra as [[s' f'] i' x' a' E3' E4' E1' E2' [Hs' Hf' Hi' Hx']].
-        by move/E3: E3' => E3''.
-      + exists s, f, (list__val__admininstr (take (size ts1) vcs) ++ [:: admininstr__TRAP]).
-        (* TODO: Can we get rid of these rewrites? *)
-        have -> : (list__val__admininstr (take (size ts1) vcs ++ [:: val__CONST (valtype__INN inn__I32) (val___inn__entry v1)]) ++ [:: admininstr__CALL_INDIRECT x]) = (list__val__admininstr (take (size ts1) vcs) ++ (list__val__admininstr [:: val__CONST (valtype__INN inn__I32) (val___inn__entry v1)] ++ [:: admininstr__CALL_INDIRECT x]) ++ [::]).
-        { rewrite cats0 catA. rewrite /list__val__admininstr. rewrite !map_map. rewrite map_cat. by []. }
-        rewrite -[[:: admininstr__TRAP]]cats0.
-        apply Step__ctxt_seq with
-          (v_admininstr := list__val__admininstr [:: val__CONST (valtype__INN inn__I32) (val___inn__entry v1)] ++ [:: admininstr__CALL_INDIRECT x]).
-        apply: Step__read.
-        apply: Step_read__call_indirect_trap.
-        move => Hcontra.
-        inversion Hcontra as [[s' f'] i' x' a' E3' E4' E1' E2' [Hs' Hf' Hi' Hx']].
-        rewrite E1 in E1'. inversion E1' as [E1''].
-        rewrite -E1'' in E2'.
-        by move/E2: E2' => E2''.
-      + exists s, f, (list__val__admininstr (take (size ts1) vcs) ++ [:: admininstr__TRAP]).
-        (* TODO: Can we get rid of these rewrites? *)
-        have -> : (list__val__admininstr (take (size ts1) vcs ++ [:: val__CONST (valtype__INN inn__I32) (val___inn__entry v1)]) ++ [:: admininstr__CALL_INDIRECT x]) = (list__val__admininstr (take (size ts1) vcs) ++ (list__val__admininstr [:: val__CONST (valtype__INN inn__I32) (val___inn__entry v1)] ++ [:: admininstr__CALL_INDIRECT x]) ++ [::]).
-        { rewrite cats0 catA. rewrite /list__val__admininstr. rewrite !map_map. rewrite map_cat. by []. }
-        rewrite -[[:: admininstr__TRAP]]cats0.
-        apply Step__ctxt_seq with
-          (v_admininstr := list__val__admininstr [:: val__CONST (valtype__INN inn__I32) (val___inn__entry v1)] ++ [:: admininstr__CALL_INDIRECT x]).
-        apply: Step__read.
-        apply: Step_read__call_indirect_trap.
-        move => Hcontra.
-        inversion Hcontra as [[s' f'] i' x' a' E3' E4' E1' E2' [Hs' Hf' Hi' Hx']].
-        by rewrite E1 in E1'.
-    - (* Instr_ok__return *)
-      (* TODO: This case should be discarded by not_lf_return *)
-      by admit.
-    - (* Instr_ok__const *)
-      move => C t vc.
-      move => s f C' vcs ts1 ts2 lab ret Htf Hcontext Hmod Hts Hstore.
-      by left. 
-    - (* Instr_ok__unop *)
-      move => C t unop.
-      move => s f C' vcs ts1 ts2 lab ret Htf Hcontext Hmod Hts Hstore.
-      right.
-      case: Htf => Htf1 _. rewrite -Htf1 in Hts. invert_typeof_vcs.
-      case: v1 Ht1 => [t1 v1] /= Ht1. rewrite Ht1.
-      case Eunop: (fun_unop t unop v1) => [c | ].
-      + exists s, f, [:: admininstr__CONST t c].
-        apply: Step__pure.
-        by apply: Step_pure__unop_val.
-      + exists s, f, [:: admininstr__TRAP].
-        apply: Step__pure.
-        by apply: Step_pure__unop_trap.
-    - (* Instr_ok__binop *)
-      move => C t binop.
-      move => s f C' vcs ts1 ts2 lab ret Htf Hcontext Hmod Hts Hstore.
-      right.
-      case: Htf => Htf1 _. rewrite -Htf1 in Hts. invert_typeof_vcs.
-      case: v1 Ht1 => [t1 v1] /= Ht1. rewrite Ht1.
-      case: v2 Ht2 => [t2 v2] /= Ht2. rewrite Ht2.
-      case Ebinop: (fun_binop t binop v1 v2) => [c | ].
-      + exists s, f, [:: admininstr__CONST t c].
-        apply: Step__pure.
-        by apply: Step_pure__binop_val.
-      + exists s, f, [:: admininstr__TRAP].
-        apply: Step__pure.
-        by apply: Step_pure__binop_trap.
-    - (* Instr_ok__testop *)
-      move => C t testop.
-      move => s f C' vcs ts1 ts2 lab ret Htf Hcontext Hmod Hts Hstore.
-      right.
-      case: Htf => Htf1 _. rewrite -Htf1 in Hts. invert_typeof_vcs.
-      case: v1 Ht1 => [t1 v1] /= Ht1. rewrite Ht1.
-      move Etestop: (fun_testop t testop v1) => c.
-      exists s, f, [:: admininstr__CONST (valtype__INN inn__I32) c].
-      move/fun_testop_returns_inn_entry: (Etestop) => [c' Hc'].
-      rewrite Hc'. rewrite Hc' in Etestop.
-      apply: Step__pure.
-      by apply: Step_pure__testop.
-    - (* Instr_ok__relop *)
-      move => C t relop.
-      move => s f C' vcs ts1 ts2 lab ret Htf Hcontext Hmod Hts Hstore.
-      right. 
-      case: Htf => Htf1 _. rewrite -Htf1 in Hts. invert_typeof_vcs.
-      case: v1 Ht1 => [t1 v1] /= Ht1. rewrite Ht1.
-      case: v2 Ht2 => [t2 v2] /= Ht2. rewrite Ht2.
-      move Erelop: (fun_relop t relop v1 v2) => c.
-      exists s, f, [:: admininstr__CONST (valtype__INN inn__I32) c].
-      move/fun_relop_returns_inn_entry: (Erelop) => [c' Hc'].
-      rewrite Hc'. rewrite Hc' in Erelop.
-      apply: Step__pure.
-      by apply: Step_pure__relop.
-    - (* Instr_ok__cvtop_reinterpret *)
-      move => C t2' t1' Hsize.
-      move => s f C' vcs ts1 ts2 lab ret Htf Hcontext Hmod Hts Hstore.
-      right.
-      case: Htf => Htf1 _. rewrite -Htf1 in Hts. invert_typeof_vcs.
-      case: v1 Ht1 => [t1 v1] /= Ht1. rewrite Ht1.
-      case Ecvtop: (fun_cvtop t1' t2' cvtop__REINTERPRET None v1) => [c | ].
-      + exists s, f, [:: admininstr__CONST t2' c].
-        apply: Step__pure.
-        by apply: Step_pure__cvtop_val.
-      + exists s, f, [:: admininstr__TRAP].
-        apply: Step__pure.
-        by apply: Step_pure__cvtop_trap.
-    - (* Instr_ok__cvtop_convert_i *)
-      move => C inn2 inn1 sx Hinn.
-      move => s f C' vcs ts1 ts2 lab ret Htf Hcontext Hmod Hts Hstore.
-      right.
-      case: Htf => Htf1 _. rewrite -Htf1 in Hts. invert_typeof_vcs.
-      case: v1 Ht1 => [t1 v1] /= Ht1. rewrite Ht1.
-      case Ecvtop: (fun_cvtop (valtype__INN inn1) (valtype__INN inn2) cvtop__CONVERT sx v1) => [c | ].
-      + exists s, f, [:: admininstr__CONST (valtype__INN inn2) c].
-        apply: Step__pure.
-        by apply: Step_pure__cvtop_val.
-      + exists s, f, [:: admininstr__TRAP].
-        apply: Step__pure.
-        by apply: Step_pure__cvtop_trap.
-    - (* Instr_ok__cvtop_convert_f *)
-      move => C fnn2 fnn1.
-      move => s f C' vcs ts1 ts2 lab ret Htf Hcontext Hmod Hts Hstore.
-      right.
-      case: Htf => Htf1 _. rewrite -Htf1 in Hts. invert_typeof_vcs.
-      case: v1 Ht1 => [t1 v1] /= Ht1. rewrite Ht1.
-      case Ecvtop: (fun_cvtop (valtype__FNN fnn1) (valtype__FNN fnn2) cvtop__CONVERT None v1) => [c | ].
-      + exists s, f, [:: admininstr__CONST (valtype__FNN fnn2) c].
-        apply: Step__pure.
-        by apply: Step_pure__cvtop_val.
-      + exists s, f, [:: admininstr__TRAP].
-        apply: Step__pure.
-        by apply: Step_pure__cvtop_trap.
-    - (* Instr_ok__local_get *)
-      move => C x t Hlen Hlookup.
-      move => s f C' vcs ts1 ts2 lab ret Htf Hcontext Hmod Hts Hstore.
-      right.
-      case: Htf => Htf1 _. rewrite -Htf1 in Hts. invert_typeof_vcs.
-      exists s, f, (list__val__admininstr [:: fun_local (state__ s f) x]).
+        (v_admininstr := list__val__admininstr [:: val__CONST (valtype__INN inn__I32) (val___inn__entry v1)] ++ [:: admininstr__CALL_INDIRECT x]%list).
       apply: Step__read.
-      by apply: Step_read__local_get.
-    - (* Instr_ok__local_set *)
-      move => C x t Hlen Hlookup.
-      move => s f C' vcs ts1 ts2 lab ret Htf Hcontext Hmod Hts Hstore.
-      right.
-      case: Htf => Htf1 _. rewrite -Htf1 in Hts. invert_typeof_vcs.
-      (* TODO: Does set/pose tactic support destructuring? *)
-      case Estate: (fun_with_local (state__ s f) x v1) => [s' f'].
-      exists s', f', [::].
-      rewrite -Estate.
-      by apply: Step__local_set.
-    - (* Instr_ok__local_tee *)
-      move => C x t Hlen Hlookup.
-      move => s f C' vcs ts1 ts2 lab ret Htf Hcontext Hmod Hts Hstore.
-      right.
-      case: Htf => Htf1 _. rewrite -Htf1 in Hts. invert_typeof_vcs.
-      exists s, f, [:: fun_coec_val__admininstr v1; fun_coec_val__admininstr v1; admininstr__LOCAL_SET x].
+      apply: Step_read__call_indirect_call => //=.
+    + exists s, f, (list__val__admininstr (take (size ts1) vcs) ++ [:: admininstr__TRAP]).
+      (* TODO: Can we get rid of these rewrites? *)
+      have -> : (list__val__admininstr (take (size ts1) vcs ++ [:: val__CONST (valtype__INN inn__I32) (val___inn__entry v1)]) ++ [:: admininstr__CALL_INDIRECT x]) = (list__val__admininstr (take (size ts1) vcs) ++ (list__val__admininstr [:: val__CONST (valtype__INN inn__I32) (val___inn__entry v1)] ++ [:: admininstr__CALL_INDIRECT x]) ++ [::]).
+      { rewrite cats0 catA. rewrite /list__val__admininstr. rewrite !map_map. rewrite map_cat. by []. }
+      rewrite -[[:: admininstr__TRAP]]cats0.
+      apply Step__ctxt_seq with
+        (v_admininstr := list__val__admininstr [:: val__CONST (valtype__INN inn__I32) (val___inn__entry v1)] ++ [:: admininstr__CALL_INDIRECT x]).
+      apply: Step__read.
+      apply: Step_read__call_indirect_trap.
+      move => Hcontra.
+      inversion Hcontra as [[s' f'] i' x' a' E3' E4' E1' E2' [Hs' Hf' Hi' Hx']].
+      rewrite E1 in E1'. inversion E1' as [E1''].
+      rewrite -E1'' in E4'.
+      by move/E4: E4' => E4''.
+    + exists s, f, (list__val__admininstr (take (size ts1) vcs) ++ [:: admininstr__TRAP]).
+      (* TODO: Can we get rid of these rewrites? *)
+      have -> : (list__val__admininstr (take (size ts1) vcs ++ [:: val__CONST (valtype__INN inn__I32) (val___inn__entry v1)]) ++ [:: admininstr__CALL_INDIRECT x]) = (list__val__admininstr (take (size ts1) vcs) ++ (list__val__admininstr [:: val__CONST (valtype__INN inn__I32) (val___inn__entry v1)] ++ [:: admininstr__CALL_INDIRECT x]) ++ [::]).
+      { rewrite cats0 catA. rewrite /list__val__admininstr. rewrite !map_map. rewrite map_cat. by []. }
+      rewrite -[[:: admininstr__TRAP]]cats0.
+      apply Step__ctxt_seq with
+        (v_admininstr := list__val__admininstr [:: val__CONST (valtype__INN inn__I32) (val___inn__entry v1)] ++ [:: admininstr__CALL_INDIRECT x]).
+      apply: Step__read.
+      apply: Step_read__call_indirect_trap.
+      move => Hcontra.
+      inversion Hcontra as [[s' f'] i' x' a' E3' E4' E1' E2' [Hs' Hf' Hi' Hx']].
+      by move/E3: E3' => E3''.
+    + exists s, f, (list__val__admininstr (take (size ts1) vcs) ++ [:: admininstr__TRAP]).
+      (* TODO: Can we get rid of these rewrites? *)
+      have -> : (list__val__admininstr (take (size ts1) vcs ++ [:: val__CONST (valtype__INN inn__I32) (val___inn__entry v1)]) ++ [:: admininstr__CALL_INDIRECT x]) = (list__val__admininstr (take (size ts1) vcs) ++ (list__val__admininstr [:: val__CONST (valtype__INN inn__I32) (val___inn__entry v1)] ++ [:: admininstr__CALL_INDIRECT x]) ++ [::]).
+      { rewrite cats0 catA. rewrite /list__val__admininstr. rewrite !map_map. rewrite map_cat. by []. }
+      rewrite -[[:: admininstr__TRAP]]cats0.
+      apply Step__ctxt_seq with
+        (v_admininstr := list__val__admininstr [:: val__CONST (valtype__INN inn__I32) (val___inn__entry v1)] ++ [:: admininstr__CALL_INDIRECT x]).
+      apply: Step__read.
+      apply: Step_read__call_indirect_trap.
+      move => Hcontra.
+      inversion Hcontra as [[s' f'] i' x' a' E3' E4' E1' E2' [Hs' Hf' Hi' Hx']].
+      rewrite E1 in E1'. inversion E1' as [E1''].
+      rewrite -E1'' in E2'.
+      by move/E2: E2' => E2''.
+    + exists s, f, (list__val__admininstr (take (size ts1) vcs) ++ [:: admininstr__TRAP]).
+      (* TODO: Can we get rid of these rewrites? *)
+      have -> : (list__val__admininstr (take (size ts1) vcs ++ [:: val__CONST (valtype__INN inn__I32) (val___inn__entry v1)]) ++ [:: admininstr__CALL_INDIRECT x]) = (list__val__admininstr (take (size ts1) vcs) ++ (list__val__admininstr [:: val__CONST (valtype__INN inn__I32) (val___inn__entry v1)] ++ [:: admininstr__CALL_INDIRECT x]) ++ [::]).
+      { rewrite cats0 catA. rewrite /list__val__admininstr. rewrite !map_map. rewrite map_cat. by []. }
+      rewrite -[[:: admininstr__TRAP]]cats0.
+      apply Step__ctxt_seq with
+        (v_admininstr := list__val__admininstr [:: val__CONST (valtype__INN inn__I32) (val___inn__entry v1)] ++ [:: admininstr__CALL_INDIRECT x]).
+      apply: Step__read.
+      apply: Step_read__call_indirect_trap.
+      move => Hcontra.
+      inversion Hcontra as [[s' f'] i' x' a' E3' E4' E1' E2' [Hs' Hf' Hi' Hx']].
+      by rewrite E1 in E1'.
+  - (* Instr_ok__return *)
+    move => C ts1 ts ts2 Hretts.
+    move => s f C' vcs ts1' ts2' lab ret Htf Hcontext Hmod Hts Hstore Hnotbr Hnotret.
+    rewrite /not_lf_return /= in Hnotret.
+    by inversion Hnotret.
+  - (* Instr_ok__const *)
+    move => C t vc.
+    move => s f C' vcs ts1 ts2 lab ret Htf Hcontext Hmod Hts Hstore Hnotbr Hnotret.
+    by left. 
+  - (* Instr_ok__unop *)
+    move => C t unop.
+    move => s f C' vcs ts1 ts2 lab ret Htf Hcontext Hmod Hts Hstore Hnotbr Hnotret.
+    right.
+    case: Htf => Htf1 _. rewrite -Htf1 in Hts. invert_typeof_vcs.
+    case: v1 Ht1 => [t1 v1] /= Ht1. rewrite Ht1.
+    case Eunop: (fun_unop t unop v1) => [c | ].
+    + exists s, f, [:: admininstr__CONST t c].
       apply: Step__pure.
-      by apply: Step_pure__local_tee.
-    - (* Instr_ok__global_get *)
-      move => C x t mut Hlen Hlookup.
-      move => s f C' vcs ts1 ts2 lab ret Htf Hcontext Hmod Hts Hstore.
-      right.
-      case: Htf => Htf1 _. rewrite -Htf1 in Hts. invert_typeof_vcs.
-      exists s, f, (list__val__admininstr [:: globalinst__VALUE (fun_global (state__ s f) x)]).
-      apply: Step__read.
-      by apply: Step_read__global_get.
-    - (* Instr_ok__global_set *)
-      move => C x t Hlen Hlookup.
-      move => s f C' vcs ts1 ts2 lab ret Htf Hcontext Hmod Hts Hstore.
-      right.
-      case: Htf => Htf1 _. rewrite -Htf1 in Hts. invert_typeof_vcs.
-      (* TODO: Does set/pose tactic support destructuring? *)
-      case Estate: (fun_with_global (state__ s f) x v1) => [s' f'].
-      exists s', f', [::].
-      rewrite -Estate.
-      by apply: Step__global_set.
-    - (* Instr_ok__memory_size *)
-      move => C mt Hlen Hlookup.
-      move => s f C' vcs ts1 ts2 lab ret Htf Hcontext Hmod Hts Hstore.
-      right.
-      case: Htf => Htf1 _. rewrite -Htf1 in Hts. invert_typeof_vcs.
-      (* TODO: This pose tactic cannot infer Inh_nat for some reason *)
-      (* pose addr := (lookup_total (moduleinst__MEMS (frame__MODULE f)) 0). *)
-      pose addr := (@lookup_total nat Inh_nat (moduleinst__MEMS (frame__MODULE f)) 0).
-      inversion Hstore as [? ? ? ? meminsts ? ? ? memts ? ? ? ? Hs ? ? ? Hmem Hs'] => {Hs'}.
-      have {}Hcontext : context__MEMS C = context__MEMS C'.
-      { rewrite Hcontext. by case: C' Hcontext Hmod => *. }
-      have {}Haddr : addr < size meminsts.
-      { inversion Hmod as [? ? ? ? ? memaddrs ? ? ? ? ? ? ? ? Hmemaddrs ? ? ? ? Hext Hexp Hs' Hf HC'] => {Hexp Hs'}.
-        rewrite /addr -Hf /=.
-        move/Forall2_lookup: Hext => [_ Hext].
-        move/(_ 0): Hext => Hext.
-        rewrite Hmemaddrs in Hext.
-        rewrite Hcontext -HC' /= in Hlen.
-        move/Hext: Hlen => {}Hext.
-        inversion Hext as [| | ? ? ? ? ? Hlen' |].
-        rewrite Hs length_size /= in Hlen'.
-        by move/ltP: Hlen' => Hlen'. }
-      have {}Hmem : Memory_instance_ok s (lookup_total meminsts addr) (lookup_total memts addr).
-      { move/Forall2_lookup: Hmem => [_ Hmem].
-        move/(_ addr): Hmem => Hmem.
-        move/ltP: Haddr => Haddr.
-        rewrite length_size in Hmem.
-        by move/(_ Haddr): Hmem => {}Hmem. }
-      inversion Hmem as [? ? ? n ? ? Hlen' ? Hs' Hlookup' Hmt'] => {Hs' Hmt'}.
-      exists s, f, [:: admininstr__CONST (valtype__INN inn__I32) (val___inn__entry n)].
-      apply: Step__read.
-      apply: Step_read__memory_size.
-      rewrite length_size in Hlen'.
-      rewrite /addr in Hlookup'.
-      by rewrite length_size /fun_mem Hs -Hlookup' Hlen'.
-    - (* Instr_ok__memory_grow *)
-      move => C mt Hlen Hlookup.
-      move => s f C' vcs ts1 ts2 lab ret Htf Hcontext Hmod Hts Hstore.
-      right.
-      case: Htf => Htf1 _. rewrite -Htf1 in Hts. invert_typeof_vcs.
-      invert_val_wf v1. rewrite /= in Ht1. rewrite Ht1.
-      set meminst1 := (fun_mem (state__ s f) 0).
-      (* TODO: Does set/pose tactic support destructuring? *)
-      case Ememinst1: meminst1 => [[limn1 limm1] bs1].
-      pose meminst2 := mkmeminst (limits__ (limn1 + v1) limm1) (bs1 ++ [:: byte__ 0]).
-      (* TODO: Does set/pose tactic support destructuring? *)
-      case Estate: (fun_with_meminst (state__ s f) 0 meminst2) => [s' f'].
-      (* NOTE: We could just use Step__memory_grow_fail but
-               we assume we can alway grow memory when it does not exceed predefined maximum size *)
-      case Elimm1: (limn1 + v1 <= limm1).
-      + exists s', f', [:: admininstr__CONST (valtype__INN inn__I32) (val___inn__entry (size (meminst__BYTES (fun_mem (state__ s f) 0)) / (64 * fun_Ki)%coq_nat))].
-        rewrite -length_size -Estate.
-        apply: Step__memory_grow_succeed.
-        apply: (growmemory__ meminst1 v1 meminst2 limn1 limm1 bs1 (limn1 + v1)) => //=.
-        by apply/leP.
-      + exists s, f, [:: admininstr__CONST (valtype__INN inn__I32) (val___inn__entry (fun_invsigned 32 (0 - 1)%coq_nat))].
-        by apply: Step__memory_grow_fail.
-    - (* Instr_ok__load *)
-      (* TODO: memop should be name as memarg *)
-      move => C t n sx memop mt inn Hlen Hsize Hlookup Halign1 Halign2 Hinn.
-      move => s f C' vcs ts1 ts2 lab ret Htf Hcontext Hmod Hts Hstore.
-      right.
-      case: Htf => Htf1 _. rewrite -Htf1 in Hts. invert_typeof_vcs.
-      invert_val_wf v1. rewrite /= in Ht1. rewrite Ht1.
-      case En: n => [n' |]; case Esx: sx => [sx' |].
-      + (* NOTE: t of t.load is expected to be inn *)
+      by apply: Step_pure__unop_val.
+    + exists s, f, [:: admininstr__TRAP].
+      apply: Step__pure.
+      by apply: Step_pure__unop_trap.
+  - (* Instr_ok__binop *)
+    move => C t binop.
+    move => s f C' vcs ts1 ts2 lab ret Htf Hcontext Hmod Hts Hstore Hnotbr Hnotret.
+    right.
+    case: Htf => Htf1 _. rewrite -Htf1 in Hts. invert_typeof_vcs.
+    case: v1 Ht1 => [t1 v1] /= Ht1. rewrite Ht1.
+    case: v2 Ht2 => [t2 v2] /= Ht2. rewrite Ht2.
+    case Ebinop: (fun_binop t binop v1 v2) => [c | ].
+    + exists s, f, [:: admininstr__CONST t c].
+      apply: Step__pure.
+      by apply: Step_pure__binop_val.
+    + exists s, f, [:: admininstr__TRAP].
+      apply: Step__pure.
+      by apply: Step_pure__binop_trap.
+  - (* Instr_ok__testop *)
+    move => C t testop.
+    move => s f C' vcs ts1 ts2 lab ret Htf Hcontext Hmod Hts Hstore Hnotbr Hnotret.
+    right.
+    case: Htf => Htf1 _. rewrite -Htf1 in Hts. invert_typeof_vcs.
+    case: v1 Ht1 => [t1 v1] /= Ht1. rewrite Ht1.
+    move Etestop: (fun_testop t testop v1) => c.
+    exists s, f, [:: admininstr__CONST (valtype__INN inn__I32) c].
+    move/fun_testop_returns_inn_entry: (Etestop) => [c' Hc'].
+    rewrite Hc'. rewrite Hc' in Etestop.
+    apply: Step__pure.
+    by apply: Step_pure__testop.
+  - (* Instr_ok__relop *)
+    move => C t relop.
+    move => s f C' vcs ts1 ts2 lab ret Htf Hcontext Hmod Hts Hstore Hnotbr Hnotret.
+    right. 
+    case: Htf => Htf1 _. rewrite -Htf1 in Hts. invert_typeof_vcs.
+    case: v1 Ht1 => [t1 v1] /= Ht1. rewrite Ht1.
+    case: v2 Ht2 => [t2 v2] /= Ht2. rewrite Ht2.
+    move Erelop: (fun_relop t relop v1 v2) => c.
+    exists s, f, [:: admininstr__CONST (valtype__INN inn__I32) c].
+    move/fun_relop_returns_inn_entry: (Erelop) => [c' Hc'].
+    rewrite Hc'. rewrite Hc' in Erelop.
+    apply: Step__pure.
+    by apply: Step_pure__relop.
+  - (* Instr_ok__cvtop_reinterpret *)
+    move => C t2' t1' Hsize.
+    move => s f C' vcs ts1 ts2 lab ret Htf Hcontext Hmod Hts Hstore Hnotbr Hnotret.
+    right.
+    case: Htf => Htf1 _. rewrite -Htf1 in Hts. invert_typeof_vcs.
+    case: v1 Ht1 => [t1 v1] /= Ht1. rewrite Ht1.
+    case Ecvtop: (fun_cvtop t1' t2' cvtop__REINTERPRET None v1) => [c | ].
+    + exists s, f, [:: admininstr__CONST t2' c].
+      apply: Step__pure.
+      by apply: Step_pure__cvtop_val.
+    + exists s, f, [:: admininstr__TRAP].
+      apply: Step__pure.
+      by apply: Step_pure__cvtop_trap.
+  - (* Instr_ok__cvtop_convert_i *)
+    move => C inn2 inn1 sx Hinn.
+    move => s f C' vcs ts1 ts2 lab ret Htf Hcontext Hmod Hts Hstore Hnotbr Hnotret.
+    right.
+    case: Htf => Htf1 _. rewrite -Htf1 in Hts. invert_typeof_vcs.
+    case: v1 Ht1 => [t1 v1] /= Ht1. rewrite Ht1.
+    case Ecvtop: (fun_cvtop (valtype__INN inn1) (valtype__INN inn2) cvtop__CONVERT sx v1) => [c | ].
+    + exists s, f, [:: admininstr__CONST (valtype__INN inn2) c].
+      apply: Step__pure.
+      by apply: Step_pure__cvtop_val.
+    + exists s, f, [:: admininstr__TRAP].
+      apply: Step__pure.
+      by apply: Step_pure__cvtop_trap.
+  - (* Instr_ok__cvtop_convert_f *)
+    move => C fnn2 fnn1.
+    move => s f C' vcs ts1 ts2 lab ret Htf Hcontext Hmod Hts Hstore Hnotbr Hnotret.
+    right.
+    case: Htf => Htf1 _. rewrite -Htf1 in Hts. invert_typeof_vcs.
+    case: v1 Ht1 => [t1 v1] /= Ht1. rewrite Ht1.
+    case Ecvtop: (fun_cvtop (valtype__FNN fnn1) (valtype__FNN fnn2) cvtop__CONVERT None v1) => [c | ].
+    + exists s, f, [:: admininstr__CONST (valtype__FNN fnn2) c].
+      apply: Step__pure.
+      by apply: Step_pure__cvtop_val.
+    + exists s, f, [:: admininstr__TRAP].
+      apply: Step__pure.
+      by apply: Step_pure__cvtop_trap.
+  - (* Instr_ok__local_get *)
+    move => C x t Hlen Hlookup.
+    move => s f C' vcs ts1 ts2 lab ret Htf Hcontext Hmod Hts Hstore Hnotbr Hnotret.
+    right.
+    case: Htf => Htf1 _. rewrite -Htf1 in Hts. invert_typeof_vcs.
+    exists s, f, (list__val__admininstr [:: fun_local (state__ s f) x]).
+    apply: Step__read.
+    by apply: Step_read__local_get.
+  - (* Instr_ok__local_set *)
+    move => C x t Hlen Hlookup.
+    move => s f C' vcs ts1 ts2 lab ret Htf Hcontext Hmod Hts Hstore Hnotbr Hnotret.
+    right.
+    case: Htf => Htf1 _. rewrite -Htf1 in Hts. invert_typeof_vcs.
+    (* TODO: Does set/pose tactic support destructuring? *)
+    case Estate: (fun_with_local (state__ s f) x v1) => [s' f'].
+    exists s', f', [::].
+    rewrite -Estate.
+    by apply: Step__local_set.
+  - (* Instr_ok__local_tee *)
+    move => C x t Hlen Hlookup.
+    move => s f C' vcs ts1 ts2 lab ret Htf Hcontext Hmod Hts Hstore Hnotbr Hnotret.
+    right.
+    case: Htf => Htf1 _. rewrite -Htf1 in Hts. invert_typeof_vcs.
+    exists s, f, [:: fun_coec_val__admininstr v1; fun_coec_val__admininstr v1; admininstr__LOCAL_SET x].
+    apply: Step__pure.
+    by apply: Step_pure__local_tee.
+  - (* Instr_ok__global_get *)
+    move => C x t mut Hlen Hlookup.
+    move => s f C' vcs ts1 ts2 lab ret Htf Hcontext Hmod Hts Hstore Hnotbr Hnotret.
+    right.
+    case: Htf => Htf1 _. rewrite -Htf1 in Hts. invert_typeof_vcs.
+    exists s, f, (list__val__admininstr [:: globalinst__VALUE (fun_global (state__ s f) x)]).
+    apply: Step__read.
+    by apply: Step_read__global_get.
+  - (* Instr_ok__global_set *)
+    move => C x t Hlen Hlookup.
+    move => s f C' vcs ts1 ts2 lab ret Htf Hcontext Hmod Hts Hstore.
+    right.
+    case: Htf => Htf1 _. rewrite -Htf1 in Hts. invert_typeof_vcs.
+    (* TODO: Does set/pose tactic support destructuring? *)
+    case Estate: (fun_with_global (state__ s f) x v1) => [s' f'].
+    exists s', f', [::].
+    rewrite -Estate.
+    by apply: Step__global_set.
+  - (* Instr_ok__memory_size *)
+    move => C mt Hlen Hlookup.
+    move => s f C' vcs ts1 ts2 lab ret Htf Hcontext Hmod Hts Hstore Hnotbr Hnotret.
+    right.
+    case: Htf => Htf1 _. rewrite -Htf1 in Hts. invert_typeof_vcs.
+    (* TODO: This pose tactic cannot infer Inh_nat for some reason *)
+    (* pose addr := (lookup_total (moduleinst__MEMS (frame__MODULE f)) 0). *)
+    pose addr := (@lookup_total nat Inh_nat (moduleinst__MEMS (frame__MODULE f)) 0).
+    inversion Hstore as [? ? ? ? meminsts ? ? ? memts ? ? ? ? Hs ? ? ? Hmem Hs'] => {Hs'}.
+    have {}Hcontext : context__MEMS C = context__MEMS C'.
+    { rewrite Hcontext. by case: C' Hcontext Hmod => *. }
+    have {}Haddr : addr < size meminsts.
+    { inversion Hmod as [? ? ? ? ? memaddrs ? ? ? ? ? ? ? ? Hmemaddrs ? ? ? ? Hext Hexp Hs' Hf HC'] => {Hexp Hs'}.
+      rewrite /addr -Hf /=.
+      move/Forall2_lookup: Hext => [_ Hext].
+      move/(_ 0): Hext => Hext.
+      rewrite Hmemaddrs in Hext.
+      rewrite Hcontext -HC' /= in Hlen.
+      move/Hext: Hlen => {}Hext.
+      inversion Hext as [| | ? ? ? ? ? Hlen' |].
+      rewrite Hs length_size /= in Hlen'.
+      by move/ltP: Hlen' => Hlen'. }
+    have {}Hmem : Memory_instance_ok s (lookup_total meminsts addr) (lookup_total memts addr).
+    { move/Forall2_lookup: Hmem => [_ Hmem].
+      move/(_ addr): Hmem => Hmem.
+      move/ltP: Haddr => Haddr.
+      rewrite length_size in Hmem.
+      by move/(_ Haddr): Hmem => {}Hmem. }
+    inversion Hmem as [? ? ? n ? ? Hlen' ? Hs' Hlookup' Hmt'] => {Hs' Hmt'}.
+    exists s, f, [:: admininstr__CONST (valtype__INN inn__I32) (val___inn__entry n)].
+    apply: Step__read.
+    apply: Step_read__memory_size.
+    rewrite length_size in Hlen'.
+    rewrite /addr in Hlookup'.
+    by rewrite length_size /fun_mem Hs -Hlookup' Hlen'.
+  - (* Instr_ok__memory_grow *)
+    move => C mt Hlen Hlookup.
+    move => s f C' vcs ts1 ts2 lab ret Htf Hcontext Hmod Hts Hstore Hnotbr Hnotret.
+    right.
+    case: Htf => Htf1 _. rewrite -Htf1 in Hts. invert_typeof_vcs.
+    invert_val_wf v1. rewrite /= in Ht1. rewrite Ht1.
+    set meminst1 := (fun_mem (state__ s f) 0).
+    (* TODO: Does set/pose tactic support destructuring? *)
+    case Ememinst1: meminst1 => [[limn1 limm1] bs1].
+    pose meminst2 := mkmeminst (limits__ (limn1 + v1) limm1) (bs1 ++ [:: byte__ 0]).
+    (* TODO: Does set/pose tactic support destructuring? *)
+    case Estate: (fun_with_meminst (state__ s f) 0 meminst2) => [s' f'].
+    (* NOTE: We could just use Step__memory_grow_fail but
+              we assume we can alway grow memory when it does not exceed predefined maximum size *)
+    case Elimm1: (limn1 + v1 <= limm1).
+    + exists s', f', [:: admininstr__CONST (valtype__INN inn__I32) (val___inn__entry (size (meminst__BYTES (fun_mem (state__ s f) 0)) / (64 * fun_Ki)%coq_nat))].
+      rewrite -length_size -Estate.
+      apply: Step__memory_grow_succeed.
+      apply: (growmemory__ meminst1 v1 meminst2 limn1 limm1 bs1 (limn1 + v1)) => //=.
+      by apply/leP.
+    + exists s, f, [:: admininstr__CONST (valtype__INN inn__I32) (val___inn__entry (fun_invsigned 32 (0 - 1)%coq_nat))].
+      by apply: Step__memory_grow_fail.
+  - (* Instr_ok__load *)
+    (* TODO: memop should be name as memarg *)
+    move => C t n sx memop mt inn Hlen Hsize Hlookup Halign1 Halign2 Hinn.
+    move => s f C' vcs ts1 ts2 lab ret Htf Hcontext Hmod Hts Hstore Hnotbr Hnotret.
+    right.
+    case: Htf => Htf1 _. rewrite -Htf1 in Hts. invert_typeof_vcs.
+    invert_val_wf v1. rewrite /= in Ht1. rewrite Ht1.
+    case En: n => [n' |]; case Esx: sx => [sx' |].
+    + (* NOTE: t of t.load is expected to be inn *)
+      case: Hinn => [Hcontra | ->] //=; first by rewrite En in Hcontra.
+      case Hcond: (((v1 + memop__OFFSET memop)%coq_nat + n' / 8)%coq_nat > size (meminst__BYTES (fun_mem (state__ s f) 0))).
+      * move/ltP: Hcond => Hcond.
+        exists s, f, [:: admininstr__TRAP].
+        apply: Step__read.
+        by apply: Step_read__load_pack_trap.
+      * move/negbT: Hcond => Hcond.
+        rewrite -leqNgt in Hcond.
+        move/list_slice_size: Hcond => Hcond.
+        move/fun_ibytes_inverse: Hcond => [c Hcond].
+        exists s, f, [:: admininstr__CONST (valtype__INN inn) (fun_ext n' (fun_size (valtype__INN inn)) sx' c)].
+        apply: Step__read.
+        by apply: Step_read__load_pack_val.
+    + move/Hsize: Esx => Hcontra.
+      by rewrite En in Hcontra.
+    + move/Hsize: En => Hcontra.
+      by rewrite Esx in Hcontra.
+    + case Hcond: (((v1 + memop__OFFSET memop)%coq_nat + fun_size t / 8)%coq_nat > size (meminst__BYTES (fun_mem (state__ s f) 0))).
+      * move/ltP: Hcond => Hcond.
+        exists s, f, [:: admininstr__TRAP].
+        apply: Step__read.
+        by apply: Step_read__load_num_trap.
+      * move/negbT: Hcond => Hcond.
+        rewrite -leqNgt in Hcond.
+        move/list_slice_size: Hcond => Hcond.
+        move/fun_bytes_inverse: Hcond => [c Hcond].
+        exists s, f, [:: admininstr__CONST t c].
+        apply: Step__read.
+        by apply: Step_read__load_num_val.
+  - (* Instr_ok__store *)
+    (* TODO: memop should be name as memarg *)
+    move => C t n memop mt inn Hlen Hlookup Halign1 Halign2 Hinn.
+    move => s f C' vcs ts1 ts2 lab ret Htf Hcontext Hmod Hts Hstore Hnotbr Hnotret.
+    right.
+    case: Htf => Htf1 _. rewrite -Htf1 in Hts. invert_typeof_vcs.
+    invert_val_wf v1. rewrite /= in Ht1. rewrite Ht1.
+    invert_val_wf v2. rewrite /= in Ht2. rewrite Ht2.
+    + case En: n => [n' |].
+      * (* NOTE: t of t.store is expected to be inn *)
         case: Hinn => [Hcontra | ->] //=; first by rewrite En in Hcontra.
         case Hcond: (((v1 + memop__OFFSET memop)%coq_nat + n' / 8)%coq_nat > size (meminst__BYTES (fun_mem (state__ s f) 0))).
-        * move/ltP: Hcond => Hcond.
+        { move/ltP: Hcond => Hcond.
           exists s, f, [:: admininstr__TRAP].
-          apply: Step__read.
-          by apply: Step_read__load_pack_trap.
-        * move/negbT: Hcond => Hcond.
-          rewrite -leqNgt in Hcond.
-          move/list_slice_size: Hcond => Hcond.
-          move/fun_ibytes_inverse: Hcond => [c Hcond].
-          exists s, f, [:: admininstr__CONST (valtype__INN inn) (fun_ext n' (fun_size (valtype__INN inn)) sx' c)].
-          apply: Step__read.
-          by apply: Step_read__load_pack_val.
-      + move/Hsize: Esx => Hcontra.
-        by rewrite En in Hcontra.
-      + move/Hsize: En => Hcontra.
-        by rewrite Esx in Hcontra.
-      + case Hcond: (((v1 + memop__OFFSET memop)%coq_nat + fun_size t / 8)%coq_nat > size (meminst__BYTES (fun_mem (state__ s f) 0))).
-        * move/ltP: Hcond => Hcond.
+          by apply: Step__store_pack_trap. }
+        { set bs := fun_ibytes n' (fun_wrap (fun_size (valtype__INN inn)) n' v2).
+          case Estate: (fun_with_mem (state__ s f) 0 (v1 + memop__OFFSET memop)%coq_nat (n' / 8) bs) => [s' f'].
+          exists s', f', [::].
+          rewrite -Estate.
+          by apply: Step__store_pack_val. }
+      * case Hcond: (((v1 + memop__OFFSET memop)%coq_nat + fun_size t / 8)%coq_nat > size (meminst__BYTES (fun_mem (state__ s f) 0))).
+        { move/ltP: Hcond => Hcond.
           exists s, f, [:: admininstr__TRAP].
-          apply: Step__read.
-          by apply: Step_read__load_num_trap.
-        * move/negbT: Hcond => Hcond.
-          rewrite -leqNgt in Hcond.
-          move/list_slice_size: Hcond => Hcond.
-          move/fun_bytes_inverse: Hcond => [c Hcond].
-          exists s, f, [:: admininstr__CONST t c].
-          apply: Step__read.
-          by apply: Step_read__load_num_val.
-    - (* Instr_ok__store *)
-      (* TODO: memop should be name as memarg *)
-      move => C t n memop mt inn Hlen Hlookup Halign1 Halign2 Hinn.
-      move => s f C' vcs ts1 ts2 lab ret Htf Hcontext Hmod Hts Hstore.
-      right.
-      case: Htf => Htf1 _. rewrite -Htf1 in Hts. invert_typeof_vcs.
-      invert_val_wf v1. rewrite /= in Ht1. rewrite Ht1.
-      invert_val_wf v2. rewrite /= in Ht2. rewrite Ht2.
-      + case En: n => [n' |].
-        * (* NOTE: t of t.store is expected to be inn *)
-          case: Hinn => [Hcontra | ->] //=; first by rewrite En in Hcontra.
-          case Hcond: (((v1 + memop__OFFSET memop)%coq_nat + n' / 8)%coq_nat > size (meminst__BYTES (fun_mem (state__ s f) 0))).
-          { move/ltP: Hcond => Hcond.
-            exists s, f, [:: admininstr__TRAP].
-            by apply: Step__store_pack_trap. }
-          { set bs := fun_ibytes n' (fun_wrap (fun_size (valtype__INN inn)) n' v2).
-            case Estate: (fun_with_mem (state__ s f) 0 (v1 + memop__OFFSET memop)%coq_nat (n' / 8) bs) => [s' f'].
-            exists s', f', [::].
-            rewrite -Estate.
-            by apply: Step__store_pack_val. }
-        * case Hcond: (((v1 + memop__OFFSET memop)%coq_nat + fun_size t / 8)%coq_nat > size (meminst__BYTES (fun_mem (state__ s f) 0))).
-          { move/ltP: Hcond => Hcond.
-            exists s, f, [:: admininstr__TRAP].
-            by apply: Step__store_num_trap. }
-          { set bs := fun_bytes t v2.
-            case Estate: (fun_with_mem (state__ s f) 0 (v1 + memop__OFFSET memop)%coq_nat (fun_size t / 8) bs) => [s' f'].
-            exists s', f', [::].
-            rewrite -Estate.
-            by apply: Step__store_num_val. }
-      + case En: n => [n' |].
-        * (* NOTE: t of t.store is expected to be inn *)
-          case: Hinn => [Hcontra | Hinn] //=; first by rewrite En in Hcontra.
-          by rewrite Hinn /= in Ht2.
-        * case Hcond: (((v1 + memop__OFFSET memop)%coq_nat + fun_size t / 8)%coq_nat > size (meminst__BYTES (fun_mem (state__ s f) 0))).
-          { move/ltP: Hcond => Hcond.
-            exists s, f, [:: admininstr__TRAP].
-            rewrite -Ht2 /= in Hcond *.
-            by apply: Step__store_num_trap. }
-          { set bs := fun_bytes t v2.
-            case Estate: (fun_with_mem (state__ s f) 0 (v1 + memop__OFFSET memop)%coq_nat (fun_size t / 8) bs) => [s' f'].
-            exists s', f', [::].
-            rewrite -Estate /=.
-            rewrite /bs -Ht2 /= in Hcond *.
-            by apply: Step__store_num_val. }
-    - (* Instrs_ok__empty *)
-      move => C s.
-      move => f C' vcs ts1 ts2 lab ret Htf Hcontext Hmod Hts Hstore.
-      by left.
-    - (* Instrs_ok__seq *)
-      move => C bes1 be2 ts1 ts2 ts3 Hinstrs1 IH1 Hinstr2 IH2.
-      move => s f C' vcs ts1' ts2' lab ret Htf Hcontext Hmod Hts Hstore.
-      have Heqtf1 : functype__ ts1 ts3 = functype__ ts1 ts3 by [].
-      have Heqts1 : ts1' = ts1 by inversion Htf.
-      rewrite Heqts1 in Hts.
-      move: (IH1 s f C' vcs ts1 ts3 lab ret Heqtf1 Hcontext Hmod Hts Hstore) => {}IH1.
-      case: IH1 => [Hconst1 | Hprog1].
-      + move/const_es_exists: Hconst1 => [vs1 Hvs1].
-        (* NOTE: Maybe we should make a separate lemma rather than reusing Val_Const_list_typing in Heqts2 *)
-        have Hadmin1 : Admin_instrs_ok s C (list__instr__admininstr bes1) (functype__ ts1 ts3).
-        { by apply: Admin_instrs_ok__instrs. }
-        rewrite Hvs1 in Hadmin1 *.
-        have Heqtf2 : functype__ ts3 ts2 = functype__ ts3 ts2 by [].
-        have Heqts2 : map typeof (vcs ++ vs1) = ts3.
-        { move/Val_Const_list_typing: Hadmin1 => Hadmin1.
-          by rewrite Hadmin1 -Hts map_map map_cat. }
-        move: (IH2 s f C' (vcs ++ vs1) ts3 ts2 lab ret Heqtf2 Hcontext Hmod Heqts2 Hstore) => {}IH2.
-        case: IH2 => [Hconst2 | Hprog2].
-        * left. rewrite -be_to_e_cat Hvs1.
-          apply: const_list_concat => //=.
-          by apply: v_to_e_const.
-        * right.
-          Set Printing Coercions.
-          rewrite -v_to_e_cat -Hvs1 in Hprog2.
-          by rewrite -catA be_to_e_cat in Hprog2.
-      + right. move: Hprog1 => [s' [f' [es1' Hprog1]]].
-        exists s', f', (es1' ++ list__instr__admininstr [:: be2]).
-        rewrite -be_to_e_cat catA.
-        by apply Step__ctxt_seq with (v_val := [::]).
-    - (* Instrs_ok__frame *)
-      move => C bes ts ts1 ts2 Hinstrs IH.
-      move => s f C' vcs ts1' ts2' lab ret Htf Hcontext Hmod Hts Hstore.
-      (* NOTE: This should be named as Instrs_ok__weakening *)
-      (* TODO: Get rid of duplicate proof *)
-      have Heqtf : functype__ ts1 ts2 = functype__ ts1 ts2 by [].
-      have Heqts : map typeof (drop (length ts) vcs) = ts1.
-      { rewrite map_drop.
-        injection Htf => Htf2 Htf1.
-        rewrite -Hts in Htf1. by rewrite -Htf1 drop_cat length_size ltnn subnn drop0. }
-      move: (IH s f C' (drop (length ts) vcs) ts1 ts2 lab ret Heqtf Hcontext Hmod Heqts Hstore) => {}IH.
-      have -> : vcs = (take (size ts) vcs ++ drop (size ts) vcs) by rewrite cat_take_drop.
-      rewrite {}length_size in IH.
-      set vcs1 := take (size ts) vcs in IH *.
-      set vcs2 := drop (size ts) vcs in IH *.
-      case: IH => [Hconst | Hprog].
-      + by left.
-      + right. move: Hprog => [s' [f' [es' IH]]].
-        exists s', f', (list__val__admininstr vcs1 ++ es').
-        rewrite -v_to_e_cat -catA.
-        (* TODO: Can we get rid of these rewrites? *)
-        rewrite -[list__val__admininstr vcs2 ++ _]cats0.
-        rewrite -[list__val__admininstr vcs1 ++ es']cats0.
-        rewrite -[(list__val__admininstr vcs1 ++ es') ++ [::]]catA.
-        by apply Step__ctxt_seq with
-          (v_admininstr := list__val__admininstr vcs2 ++ list__instr__admininstr bes)
-          (v_admininstr' := es')
-          (v_admininstr'' := [::]).
-Admitted.
+          by apply: Step__store_num_trap. }
+        { set bs := fun_bytes t v2.
+          case Estate: (fun_with_mem (state__ s f) 0 (v1 + memop__OFFSET memop)%coq_nat (fun_size t / 8) bs) => [s' f'].
+          exists s', f', [::].
+          rewrite -Estate.
+          by apply: Step__store_num_val. }
+    + case En: n => [n' |].
+      * (* NOTE: t of t.store is expected to be inn *)
+        case: Hinn => [Hcontra | Hinn] //=; first by rewrite En in Hcontra.
+        by rewrite Hinn /= in Ht2.
+      * case Hcond: (((v1 + memop__OFFSET memop)%coq_nat + fun_size t / 8)%coq_nat > size (meminst__BYTES (fun_mem (state__ s f) 0))).
+        { move/ltP: Hcond => Hcond.
+          exists s, f, [:: admininstr__TRAP].
+          rewrite -Ht2 /= in Hcond *.
+          by apply: Step__store_num_trap. }
+        { set bs := fun_bytes t v2.
+          case Estate: (fun_with_mem (state__ s f) 0 (v1 + memop__OFFSET memop)%coq_nat (fun_size t / 8) bs) => [s' f'].
+          exists s', f', [::].
+          rewrite -Estate /=.
+          rewrite /bs -Ht2 /= in Hcond *.
+          by apply: Step__store_num_val. }
+  - (* Instrs_ok__empty *)
+    move => C s.
+    move => f C' vcs ts1 ts2 lab ret Htf Hcontext Hmod Hts Hstore Hnotbr Hnotret.
+    by left.
+  - (* Instrs_ok__seq *)
+    move => C bes1 be2 ts1 ts2 ts3 Hinstrs1 IH1 Hinstr2 IH2.
+    move => s f C' vcs ts1' ts2' lab ret Htf Hcontext Hmod Hts Hstore Hnotbr Hnotret.
+    (* MEMO: This is failing because of Hnotbr and Hnotret in IH *)
+    have Heqtf1 : functype__ ts1 ts3 = functype__ ts1 ts3 by [].
+    have Heqts1 : ts1' = ts1 by inversion Htf.
+    rewrite Heqts1 in Hts.
+    rewrite cat_app -be_to_e_cat in Hnotbr Hnotret.
+    move/not_lf_br_cat: Hnotbr => [Hnotbr1 Hnotbr2].
+    move/not_lf_return_cat: Hnotret => [Hnotret1 Hnotret2].
+    move: (IH1 s f C' vcs ts1 ts3 lab ret Heqtf1 Hcontext Hmod Hts Hstore Hnotbr1 Hnotret1) => {}IH1.
+    case: IH1 => [Hconst1 | Hprog1].
+    + move/const_es_exists: Hconst1 => [vs1 Hvs1].
+      (* NOTE: Maybe we should make a separate lemma rather than reusing Val_Const_list_typing in Heqts2 *)
+      have Hadmin1 : Admin_instrs_ok s C (list__instr__admininstr bes1) (functype__ ts1 ts3).
+      { by apply: Admin_instrs_ok__instrs. }
+      rewrite Hvs1 in Hadmin1 *.
+      have Heqtf2 : functype__ ts3 ts2 = functype__ ts3 ts2 by [].
+      have Heqts2 : map typeof (vcs ++ vs1) = ts3.
+      { move/Val_Const_list_typing: Hadmin1 => Hadmin1.
+        by rewrite Hadmin1 -Hts map_map map_cat. }
+      move: (IH2 s f C' (vcs ++ vs1) ts3 ts2 lab ret Heqtf2 Hcontext Hmod Heqts2 Hstore Hnotbr2 Hnotret2) => {}IH2.
+      case: IH2 => [Hconst2 | Hprog2].
+      * left. rewrite -be_to_e_cat Hvs1.
+        apply: const_list_concat => //=.
+        by apply: v_to_e_const.
+      * right.
+        rewrite -v_to_e_cat -Hvs1 in Hprog2.
+        by rewrite -catA be_to_e_cat in Hprog2.
+    + right. move: Hprog1 => [s' [f' [es1' Hprog1]]].
+      exists s', f', (es1' ++ list__instr__admininstr [:: be2]).
+      rewrite -be_to_e_cat catA.
+      by apply Step__ctxt_seq with (v_val := [::]).
+  - (* Instrs_ok__frame *)
+    move => C bes ts ts1 ts2 Hinstrs IH.
+    move => s f C' vcs ts1' ts2' lab ret Htf Hcontext Hmod Hts Hstore Hnotbr Hnotret.
+    (* NOTE: This should be named as Instrs_ok__weakening *)
+    (* TODO: Get rid of duplicate proof *)
+    have Heqtf : functype__ ts1 ts2 = functype__ ts1 ts2 by [].
+    have Heqts : map typeof (drop (length ts) vcs) = ts1.
+    { rewrite map_drop.
+      injection Htf => Htf2 Htf1.
+      rewrite -Hts in Htf1. by rewrite -Htf1 drop_cat length_size ltnn subnn drop0. }
+    move: (IH s f C' (drop (length ts) vcs) ts1 ts2 lab ret Heqtf Hcontext Hmod Heqts Hstore Hnotbr Hnotret) => {}IH.
+    have -> : vcs = (take (size ts) vcs ++ drop (size ts) vcs) by rewrite cat_take_drop.
+    rewrite {}length_size in IH.
+    set vcs1 := take (size ts) vcs in IH *.
+    set vcs2 := drop (size ts) vcs in IH *.
+    case: IH => [Hconst | Hprog].
+    + by left.
+    + right. move: Hprog => [s' [f' [es' IH]]].
+      exists s', f', (list__val__admininstr vcs1 ++ es').
+      rewrite -v_to_e_cat -catA.
+      (* TODO: Can we get rid of these rewrites? *)
+      rewrite -[list__val__admininstr vcs2 ++ _]cats0.
+      rewrite -[list__val__admininstr vcs1 ++ es']cats0.
+      rewrite -[(list__val__admininstr vcs1 ++ es') ++ [::]]catA.
+      by apply Step__ctxt_seq with
+        (v_admininstr := list__val__admininstr vcs2 ++ list__instr__admininstr bes)
+        (v_admininstr' := es')
+        (v_admininstr'' := [::]).
+  (* TODO: These goals are shelved by Instr_ok__call_indirect for some reason *)
+  Unshelve.
+  - apply: Build_Inhabited.
+    by apply: None.
+  - apply: Build_Inhabited.
+    pose functype := functype__ [::] [::].
+    pose modinst := mkmoduleinst [::] [::] [::] [::] [::] [::].
+    pose func := func__FUNC 0 [::] [::].
+    by apply: (mkfuncinst functype modinst func).
+Qed.
 
 Lemma Instr_ok_Instrs_ok: forall C be tf,
   Instr_ok C be tf -> Instrs_ok C [:: be] tf.
